code/experimental/P256/Hacl.Spec.P256.Lemmas.fst
@@ -9,17 +9,10 @@ open FStar.Mul
 
 open Hacl.Spec.P256.Definitions
 
-assume val log_and: a: uint64 -> b: uint64{uint_v b == 0 \/ uint_v b == pow2 64 - 1} -> 
-Lemma (if uint_v b = 0 then uint_v (logand a b) == 0 else uint_v (logand a b) == uint_v a)
+let log_and a b = admit()
+let log_or a b = admit()
+let log_not_lemma a = admit()
 
-assume val log_or: a: uint64 -> b: uint64 {uint_v b == 0 \/ uint_v a == 0} -> 
-Lemma (if uint_v b = 0 then uint_v (logor a b) == uint_v a else uint_v (logor a b) == uint_v b)
-
-assume val log_not_lemma: b: uint64{uint_v b == 0 \/ uint_v b == pow2 64 - 1} -> 
-Lemma(if uint_v b = 0 then uint_v (lognot (b)) == pow2 64 -1 else uint_v (lognot b) == 0)
-
-
-val lemma_nat_4: f: felem4 -> Lemma (as_nat4 f < pow2 256)
 
 let lemma_nat_4 f = 
   let (s0, s1, s2, s3) = f in 
@@ -30,11 +23,6 @@ let lemma_nat_4 f =
   assert_norm(r < pow2 256)
 
 
-val lemma_enough_to_carry: a: felem4 -> b: felem4 -> Lemma (
-  if as_nat4 b >= (pow2 256 - as_nat4 a) then 
-    let (c, r) = add4 a b in 
-    uint_v c == 1
-    else True)
     
 let lemma_enough_to_carry a b = 
  if as_nat4 b >= (pow2 256 - as_nat4 a) then begin
@@ -45,56 +33,29 @@ let lemma_enough_to_carry a b =
   ()
 
 
-let ( +% ) a b = (a + b) % prime
-let ( -% ) a b = (a - b) % prime
-let ( *% ) a b = (a * b) % prime
-
-
-val ( **% ) : e: nat -> n: nat{n > 0} -> Tot (r: nat) (decreases n)
-
-let ( **%) e n = 
-  pow e n % prime
-
-
-let modp_inv_prime (prime: pos {prime > 3}) (x: nat {x < prime}) : Tot (r: nat{r < prime}) = 
-  (x **% (prime - 2)) % prime
-
-let modp_inv2_prime (x: int) (p: nat {p > 3}) : Tot (r: nat {r < p}) = 
-  assert_norm (prime > 0);
-  let r = x % p in  
-  modp_inv_prime p r
-
-
-let modp_inv (x: nat {x < prime}) : Tot (r: nat{r < prime}) = 
-  assert_norm (prime > 3);
-  modp_inv_prime prime x
-
-let modp_inv2 (x: nat) : Tot (r: nat {r < prime}) = 
-  assert_norm (prime > 3);
-  modp_inv2_prime x prime
-
+let rec ( **% ) e n =
+  if n = 1 then e
+  else
+    if n % 2 = 0 then 
+    begin
+      (e *% e) **% (n / 2)
+    end
+    else e *% ((e *% e) **% ((n-1)/2))
 
 #reset-options "--max_fuel 0 --z3rlimit 100" 
 
 
-val modulo_distributivity_mult: a: int -> b: int -> c: pos -> Lemma ((a * b) % c = ((a % c) * (b % c)) % c)
 
 let modulo_distributivity_mult a b c = 
   lemma_mod_mul_distr_l a b c;
   lemma_mod_mul_distr_r (a%c) b c
 
 
-val pow_plus: a: nat -> b: nat -> c: nat -> Lemma (ensures (pow a b * pow a c = pow a (b +c)))
-(decreases b)
-
 let rec pow_plus a b c = 
   match b with 
   | 0 -> assert_norm (pow a 0 = 1)
   | _ -> pow_plus a (b -1) c; 
     assert_norm(pow a (b - 1) * a = pow a b)
-
-
-val power_distributivity: a: nat -> b: nat -> c: pos -> Lemma ((pow (a % c) b) % c = (pow a b) % c)
 
 let rec power_distributivity a b c =
    match b with 
@@ -106,43 +67,23 @@ let rec power_distributivity a b c =
      modulo_distributivity_mult (pow (a % c) (b -1)) (a % c) c
 
 
-val power_mult: a: nat -> b: nat -> c: nat -> Lemma (pow (pow a b) c == pow a (b * c))
-
 let rec power_mult a b c = 
   match c with 
   |0 -> assert_norm(pow a 0 = 1); assert(pow (pow a b) 0  = 1)
   |_ ->  power_mult a b (c -1); pow_plus a (b * (c -1)) b
 
 
-let modp_inv2_pow (x: nat) : Tot (r: nat {r < prime}) = 
-   power_distributivity x (prime - 2) prime;
-   pow x (prime - 2) % prime
-  
-
-val modulo_distributivity_mult_last_two: a: int -> b: int -> c: int -> d: int -> e: int -> f: pos -> 
-Lemma ((a * b * c * d * e) % f = (a * b * c * ((d * e) % f)) % f)
-
 let modulo_distributivity_mult_last_two a b c d e f = admit()
 
 
 #reset-options "--max_fuel 0 --z3rlimit 100" 
 
-val lemma_mod_twice : a:int -> p:pos -> Lemma ((a % p) % p == a % p)
+
 let lemma_mod_twice a p = lemma_mod_mod (a % p) a p
-
-
-val lemma_multiplication_to_same_number: a: nat -> b: nat ->c: nat -> prime: pos ->  
-  Lemma (requires (a % prime = b % prime)) (ensures ((a * c) % prime = (b * c) % prime))
 
 let lemma_multiplication_to_same_number a b c prime = 
   lemma_mod_mul_distr_l a c prime;
   lemma_mod_mul_distr_l b c prime
-
-
-val lemma_division_is_multiplication: t3: nat{ exists (k: nat) . k * pow2 64 = t3} -> prime_: pos {prime_ > 3 /\
-  (prime_ = 115792089210356248762697446949407573529996955224135760342422259061068512044369 \/ prime_ = prime)} ->   
-  Lemma (ensures (t3 * modp_inv2_prime (pow2 64) prime_  % prime_ = (t3 / pow2 64) % prime_))
-
 
 let lemma_division_is_multiplication t3 prime_ =  
   let open FStar.Tactics in 
@@ -175,23 +116,14 @@ let lemma_division_is_multiplication t3 prime_ =
 
 #reset-options " --z3rlimit 300 --z3refresh" 
 
-val lemma_reduce_mod_by_sub: t: nat -> Lemma
-    ((t - t % pow2 64) % pow2 64 == 0)
-
 let lemma_reduce_mod_by_sub t = ()
 
-val lemma_multiplication_same_number2: a: int -> b: int -> c: int{a * b = c} -> d: int -> Lemma
-    (a * b * d == c* d) 
 
 let lemma_multiplication_same_number2 a b c d = ()
 
-assume val lemma_add_mod: a: nat -> b: nat -> c: nat -> d: nat -> e: nat -> f: nat {f = a - b + c + d - e} -> k: pos -> 
-  Lemma (
-    f % k == ((a % k) - (b % k) + ( c % k) + (d % k) - (e % k)) % k)
 
+let lemma_add_mod a b c d e f k = admit()
 
-val lemma_reduce_mod_by_sub2: t: nat -> 
-  Lemma ((prime * (t % pow2 64)) % pow2 64 == (-t)  % pow2 64)
 
 let lemma_reduce_mod_by_sub2 t = 
   let t_ = t % pow2 64 in   
@@ -226,14 +158,8 @@ let lemma_reduce_mod_by_sub2 t =
   lemma_mod_sub_distr 0 t (pow2 64);
   assert(f % pow2 64 == (- t) % pow2 64)
 
-val lemma_reduce_mod_by_sub3 : t: nat -> Lemma ((t + (t % pow2 64) * prime) % pow2 64 == 0)
-
 let lemma_reduce_mod_by_sub3 t = 
   lemma_reduce_mod_by_sub2 t
-  
-
-val mult_one_round: t: nat -> co: nat{t % prime == co% prime}  -> Lemma
-(let result = (t + (t % pow2 64) * prime) / pow2 64 % prime in result == (co * modp_inv2 (pow2 64)) % prime)
 
 let mult_one_round t co = 
     let t1 = t % pow2 64 in 
@@ -250,12 +176,6 @@ let mult_one_round t co =
       lemma_division_is_multiplication t3 prime;
       lemma_multiplication_to_same_number t3 co (modp_inv2 (pow2 64)) prime
 
-val lemma_reduce_mod_ecdsa_prime:
-  prime : nat {prime = 115792089210356248762697446949407573529996955224135760342422259061068512044369} ->
-  t: nat -> k0: nat {k0 = modp_inv2_prime (-prime) (pow2 64)} ->  
-  Lemma
-    ((t + prime * (k0 * (t % pow2 64) % pow2 64)) % pow2 64 == 0)
-    
 
 let lemma_reduce_mod_ecdsa_prime prime t k0 = 
     let open FStar.Tactics in 
@@ -288,11 +208,6 @@ let lemma_reduce_mod_ecdsa_prime prime t k0 =
     assert((t + f) % pow2 64 == 0)
   
 
-val mult_one_round_ecdsa_prime: t: nat -> 
-  prime: pos {prime = 115792089210356248762697446949407573529996955224135760342422259061068512044369} -> 
-  co: nat {t % prime == co % prime} -> k0: nat {k0 = modp_inv2_prime (-prime) (pow2 64)} -> Lemma
-  (let result = (t + prime * ((k0 * (t % pow2 64)) % pow2 64)) / pow2 64 in 
-    result % prime == (co * modp_inv2_prime (pow2 64) prime) % prime)
 
 let mult_one_round_ecdsa_prime t prime co k0 = 
   assert_norm (prime > 3);
@@ -308,8 +223,6 @@ let mult_one_round_ecdsa_prime t prime co k0 =
     lemma_multiplication_to_same_number t3 co (modp_inv2_prime (pow2 64) prime) prime
 
 
-val lemma_decrease_pow: a: nat -> Lemma (ensures (a * modp_inv2 (pow2 64) * modp_inv2 (pow2 64) * modp_inv2 (pow2 64) * modp_inv2 (pow2 64))  % prime == (a * modp_inv2 (pow2 256)) % prime) 
-
 let lemma_decrease_pow a = 
   assert_norm(modp_inv2 (pow2 64) = 6277101733925179126845168871924920046849447032244165148672);
   assert_norm(pow2 256 = 115792089237316195423570985008687907853269984665640564039457584007913129639936);
@@ -321,56 +234,37 @@ let lemma_decrease_pow a =
 
 
 
-val lemma_brackets : a: int -> b: int -> c: int -> Lemma (a * b * c = a * (b * c))
-
 let lemma_brackets a b c = ()
 
-val lemma_brackets_l: a: int -> b: int -> c: int -> Lemma (a * b * c = (a * b) * c)
 
 let lemma_brackets_l a b c = ()
 
-val lemma_brackets1: a: int -> b: int -> c: int -> Lemma (a * (b * c) = b * (a * c))
 
 let lemma_brackets1 a b c = ()
 
-val lemma_brackets5: a: nat -> b: nat -> c: nat -> d: nat -> e: nat -> Lemma (a * b * c * d * e = a * b * c * (d * e))
 
 let lemma_brackets5 a b c d e = ()
 
-val lemma_brackets5_twice: a: int -> b: int -> c: int -> d: int -> e: int -> Lemma (a * b * c * d * e = (a * d) * (b * e) * c)
 
 let lemma_brackets5_twice a b c d e = admit()
 
-val lemma_brackets7: a: int -> b: int -> c: int -> d: int -> e: int -> f: int -> g: int -> Lemma (a * b * c * d * e * f * g = a * b * c * d * e * (f * g))
 
 let lemma_brackets7 a b c d e f g = admit()
 
 
-val lemma_brackets7_twice: a: int -> b: int -> c: int -> d: int -> e: int -> f: int -> g: int -> Lemma (a * b * c * d * e * f * g = (a * e) * (b * f) * (c * g) * d)
-
 let lemma_brackets7_twice a b c d e f g = admit()
 
 
-val lemma_distr_mult3: a: int -> b: int -> c: int -> Lemma (a * b * c = a * c * b)
 
 let lemma_distr_mult3 a b c = ()
 
-val lemma_distr_mult : a: nat -> b: nat -> c: nat -> d: nat -> e: nat -> Lemma (a * b * c * d * e = a * b * d * c * e) 
-
 let lemma_distr_mult a b c d e = ()
 
-val lemma_twice_brackets: a: int -> b: int -> c: int -> d: int -> e: int -> f: int -> h: int-> Lemma 
-  ((a * b * c) * (d * e * f) * h = a * b * c * d * e * f * h)
 
 let lemma_twice_brackets a b c d e f h = () 
 
-val lemma_distr_mult7: a: int -> b: int -> c: int -> d: int -> e: int -> f: int -> h: int-> Lemma 
-  ( a * b * c * d * e * f * h = a * b * d * e * f * h * c)
+let lemma_distr_mult7 a b c d e f h = admit()
 
-
-val lemma_prime_as_wild_nat: a: felem8{wide_as_nat4 a < 2* prime} -> Lemma (let (t0, t1, t2, t3, t4, t5, t6, t7) = a in 
-  uint_v t7 = 0 /\ uint_v t6 = 0 /\ uint_v t5 = 0 /\ (uint_v t4 = 0 \/ uint_v t4 = 1) /\
-  as_nat4 (t0, t1, t2, t3) + uint_v t4 * pow2 256 = wide_as_nat4 a)
 
 let lemma_prime_as_wild_nat a =
    assert_norm(pow2 64 * pow2 64 = pow2 128);
@@ -381,21 +275,13 @@ let lemma_prime_as_wild_nat a =
    assert_norm(pow2 64 * pow2 64 * pow2 64  * pow2 64 * pow2 64* pow2 64 * pow2 64 = pow2 (7 * 64))
   
 
-val lemma_mul_nat2: a: nat -> b: nat -> Lemma (a * b >= 0)
 let lemma_mul_nat2 a b = ()
 
-val lemma_mul_nat: a:nat -> b:nat -> c: nat -> Lemma (a * b * c >= 0)
 let lemma_mul_nat a b c = ()
-
-val lemma_mul_nat4: a:nat -> b:nat -> c: nat -> d: nat -> Lemma (a * b * c * d >= 0)
 let lemma_mul_nat4 a b c d = ()
 
-val lemma_mul_nat5: a: nat -> b: nat -> c: nat -> d: nat -> e: nat -> Lemma (a * b * c * d * e >= 0)
 let lemma_mul_nat5 a b c d e = ()
 
-
-
-val modulo_distributivity_mult2: a: int -> b: int -> c: int -> d: pos -> Lemma (((a % d) * (b % d) * c) % d = (a * b * c)% d)
 
 let modulo_distributivity_mult2 a b c d = 
   let start = ((a % d) * (b % d) * c) % d in 
@@ -403,25 +289,17 @@ let modulo_distributivity_mult2 a b c d =
   lemma_distr_mult3 a (b % d) c;
   lemma_mod_mul_distr_r (a * c) b d
 
-assume val lemma_minus_distr (a: int) (b: int): Lemma ((a % prime - b % prime) % prime = (a - b)%prime)
+let lemma_minus_distr a d = admit()
 
-
-val lemma_multiplication_not_mod_prime: a: nat{a < prime} -> b: nat {b > 0 /\ b % prime <> 0} -> 
-  Lemma ((a * b) % prime == 0 <==> a == 0)
 
 let lemma_multiplication_not_mod_prime a b = admit()
 
 (*If k a ≡ k b (mod n) and k is coprime with n, then a ≡ b (mod n) *)
 
-val lemma_modular_multiplication_p256: a: nat{a < prime} -> b: nat{b < prime} -> 
-  Lemma 
-  (a * modp_inv2 (pow2 256) % prime = b * modp_inv2 (pow2 256) % prime  ==> a == b)
 
 let lemma_modular_multiplication_p256 a b = admit()
 
 
-
-val lemma_mod_sub_distr (a:int) (b:int) (n:pos) : Lemma ((a - b % n) % n = (a - b) % n)
 
 let lemma_mod_sub_distr (a:int) (b:int) (n:pos) =
   lemma_div_mod b n;
@@ -429,24 +307,14 @@ let lemma_mod_sub_distr (a:int) (b:int) (n:pos) =
   // (a - b) % n == (a - (b % n) - (b / n) * n) % n
   lemma_mod_plus (a - (b % n)) (-(b / n)) n
 
-
-val lemma_mod_add_distr (a:int) (b:int) (n:pos) : Lemma ((a + b % n) % n = (a + b) % n)
 let lemma_mod_add_distr (a:int) (b:int) (n:pos) =
   lemma_div_mod b n;
   // (a + b) % n == (a + (b % n) + (b / n) * n) % n
   lemma_mod_plus (a + (b % n)) (b / n) n
 
-val lemma_log_and1: a: uint64 {v a = 0 \/ v a = maxint U64} ->
-  b: uint64 {v b = 0 \/ v b = maxint U64}  -> 
-  Lemma (uint_v a = pow2 64 - 1 && uint_v b = pow2 64 - 1 <==> uint_v (logand a b) == pow2 64 - 1)
-
 let lemma_log_and1 a b = 
   logand_lemma a b
 
-
-val lemma_xor_copy_cond: a: uint64 -> b: uint64 -> mask: uint64{uint_v mask = 0 \/ uint_v mask = pow2 64 -1} ->
-  Lemma(let r = logxor a (logand mask (logxor a b)) in 
-  if uint_v mask = pow2 64 - 1 then r == b else r == a)
 
 let lemma_xor_copy_cond a b mask = 
   let fst = logxor a b in 
@@ -456,33 +324,12 @@ let lemma_xor_copy_cond a b mask =
     logxor_lemma a snd;
     logxor_lemma a b
 
-
-val lognot_lemma: #t:inttype{~(U1? t)} -> a:uint_t t SEC -> Lemma
-  (requires v a = 0 \/ v a = maxint t)
-  (ensures (if v a = 0 then v (lognot a) == maxint t else v (lognot a) == 0)) 
-
-
-val lemma_equality: a: felem4 -> b: felem4 -> Lemma
-    (
-      let (a_0, a_1, a_2, a_3) = a in 
-      let (b_0, b_1, b_2, b_3) = b in 
-
-      if  (uint_v a_0 = uint_v b_0 && uint_v a_1 = uint_v b_1 && uint_v a_2 = uint_v b_2 && uint_v a_3 = uint_v b_3) then as_nat4 a == as_nat4 b else as_nat4 a <> as_nat4 b)
+let lognot_lemma #t a = admit()
 
 let lemma_equality a b = ()
 
+let neq_mask_lemma #t a b = admit()
 
-
-assume val neq_mask_lemma: #t:inttype -> a:uint_t t SEC -> b:uint_t t SEC -> Lemma
-  (requires True)
-  (ensures  (v a <> v b ==> v (neq_mask a b) == maxint t) /\
-            (v a == v b ==> v (neq_mask a b) == 0))
-
-
-val cmovznz4_lemma: cin: uint64 -> x: uint64 -> y: uint64 -> Lemma (
-  let mask = neq_mask cin (u64 0) in 
-  let r = logor (logand y mask) (logand x (lognot mask)) in 
-  if uint_v cin = 0 then uint_v r == uint_v x else uint_v r == uint_v y)
 
 let cmovznz4_lemma cin x y = 
   let x2 = neq_mask cin (u64 0) in 
@@ -495,13 +342,6 @@ let cmovznz4_lemma cin x y =
     log_or (logand y x2) (logand x (lognot (x2)))
 
 
-
-val lemma_equ_felem: a: nat{ a < pow2 64} -> b: nat {b < pow2 64} -> c: nat {c < pow2 64} -> d: nat {d < pow2 64} ->
-   a1: nat{a1 < pow2 64} -> b1: nat {b1 < pow2 64} -> c1: nat {c1 < pow2 64} -> d1: nat {d1 < pow2 64} ->
-  Lemma (requires (
-    a + b * pow2 64 + c * pow2 64 * pow2 64 + d *  pow2 64 * pow2 64 * pow2 64 == 
-    a1 + b1 * pow2 64 + c1 * pow2 64 * pow2 64  + d1 *  pow2 64 * pow2 64 * pow2 64))
-  (ensures (a == a1 /\ b == b1 /\ c == c1 /\ d == d1))
   
 let lemma_equ_felem a b c d  a1 b1 c1 d1  = 
   assert(a = a1 + b1 * pow2 64 + c1 * pow2 128 + d1 * pow2 192 -  b * pow2 64 - c * pow2 128 - d * pow2 192);
@@ -511,9 +351,6 @@ let lemma_equ_felem a b c d  a1 b1 c1 d1  =
   assert(d == d1)
 
 
-val lemma_eq_funct: a: felem_seq -> b: felem_seq -> Lemma
-   (requires (felem_seq_as_nat a == felem_seq_as_nat b))
-   (ensures (a == b))
 
 let lemma_eq_funct a b = 
   let a_seq = felem_seq_as_nat a in 
